Logic/Modal/Standard/Geach.lean
@@ -24,42 +24,48 @@ open System
 
 namespace AxiomSet
 
-def Geach (l : Axioms.Geach.Taple) : AxiomSet α := { Axioms.Geach l p | (p) }
+abbrev Geach (l : Axioms.Geach.Taple) : AxiomSet α := { Axioms.Geach l p | (p) }
 notation:max "𝐠𝐞(" t ")" => AxiomSet.Geach t
 
-class IsGeachAxiom (Λ : AxiomSet α) where
+class IsGeach (Λ : AxiomSet α) where
   taple : Axioms.Geach.Taple
   char : Λ = AxiomSet.Geach taple := by rfl
 
-@[simp] instance : IsGeachAxiom (𝐓 : AxiomSet α) where taple := ⟨0, 0, 1, 0⟩;
+instance : IsGeach (α := α) 𝐓 where taple := ⟨0, 0, 1, 0⟩;
 
-@[simp] instance : IsGeachAxiom (𝐁 : AxiomSet α) where taple := ⟨0, 1, 0, 1⟩;
+instance : IsGeach (α := α) 𝐁 where taple := ⟨0, 1, 0, 1⟩;
 
-@[simp] instance : IsGeachAxiom (𝐃 : AxiomSet α) where taple := ⟨0, 0, 1, 1⟩;
+instance : IsGeach (α := α) 𝐃 where taple := ⟨0, 0, 1, 1⟩;
 
-@[simp] instance : IsGeachAxiom (𝟒 : AxiomSet α) where taple := ⟨0, 2, 1, 0⟩;
+instance : IsGeach (α := α) 𝟒 where taple := ⟨0, 2, 1, 0⟩;
 
-@[simp] instance : IsGeachAxiom (𝟓 : AxiomSet α) where taple := ⟨1, 1, 0, 1⟩;
+instance : IsGeach (α := α) 𝟓 where taple := ⟨1, 1, 0, 1⟩;
 
-@[simp] instance : IsGeachAxiom (.𝟐 : AxiomSet α) where taple := ⟨1, 1, 1, 1⟩;
+instance : IsGeach (α := α) .𝟐 where taple := ⟨1, 1, 1, 1⟩;
 
-@[simp] instance : IsGeachAxiom (𝐂𝟒 : AxiomSet α) where taple := ⟨0, 1, 2, 0⟩;
+instance : IsGeach (α := α) 𝐂𝟒 where taple := ⟨0, 1, 2, 0⟩;
 
-@[simp] instance : IsGeachAxiom (𝐂𝐃 : AxiomSet α) where taple := ⟨1, 1, 0, 0⟩;
+instance : IsGeach (α := α) 𝐂𝐃 where taple := ⟨1, 1, 0, 0⟩;
 
-@[simp]
+
 def GeachLogic : List Axioms.Geach.Taple → AxiomSet α
   | [] => 𝐊
-  | x :: xs => (AxiomSet.GeachLogic xs) ∪ (AxiomSet.Geach x)
+  | x :: xs => (AxiomSet.Geach x) ∪ (AxiomSet.GeachLogic xs)
 notation:max "𝐆𝐞(" l ")" => AxiomSet.GeachLogic l
 
 namespace GeachLogic
 
 @[simp]
+lemma def_nil : 𝐆𝐞([]) = (𝐊 : AxiomSet α) := by simp [GeachLogic]
+
+@[simp]
+lemma iff_cons : 𝐆𝐞(x :: l) = (𝐠𝐞(x) : AxiomSet α) ∪ 𝐆𝐞(l) := by simp only [GeachLogic];
+
+@[simp]
 lemma subsetK : (𝐊 : AxiomSet α) ⊆ 𝐆𝐞(l) := by
   induction l with
   | nil => simp;
-  | cons => simp; apply Set.subset_union_of_subset_left (by assumption);
+  | cons => simp; apply Set.subset_union_of_subset_right (by assumption);
 
 lemma subsetK' (h : 𝐆𝐞(l) ⊆ Λ): 𝐊 ⊆ Λ := Set.Subset.trans GeachLogic.subsetK h
 
@@ -69,27 +75,25 @@ end GeachLogic
 
 class IsGeachLogic (Λ : AxiomSet α) where
   taples : List Axioms.Geach.Taple
-  char : Λ = 𝐆𝐞(taples) := by simp; rfl;
+  char : Λ = 𝐆𝐞(taples) := by aesop;
 
 instance [Λ.IsGeachLogic] : System.K Λ := by rw [IsGeachLogic.char (Λ := Λ)]; exact GeachLogic.instK;
 
-@[simp] instance : IsGeachLogic (𝐊 : AxiomSet α) where
-  taples := [];
-  char := by simp;
+instance : IsGeachLogic (α := α) 𝐊 where taples := [];
 
-@[simp] instance : IsGeachLogic (𝐊𝐃 : AxiomSet α) where taples := [⟨0, 0, 1, 1⟩]
+instance : IsGeachLogic (α := α) 𝐊𝐃 where taples := [⟨0, 0, 1, 1⟩]
 
-@[simp] instance : IsGeachLogic (𝐊𝐓 : AxiomSet α) where taples := [⟨0, 0, 1, 0⟩]
+instance : IsGeachLogic (α := α) 𝐊𝐓 where taples := [⟨0, 0, 1, 0⟩]
 
-@[simp] instance : IsGeachLogic (𝐊𝟒 : AxiomSet α) where taples := [⟨0, 2, 1, 0⟩]
+instance : IsGeachLogic (α := α) 𝐊𝟒 where taples := [⟨0, 2, 1, 0⟩]
 
-@[simp] instance : IsGeachLogic (𝐒𝟒 : AxiomSet α) where taples := [⟨0, 0, 1, 0⟩, ⟨0, 2, 1, 0⟩].reverse
+instance : IsGeachLogic (α := α) 𝐒𝟒 where taples := [⟨0, 0, 1, 0⟩, ⟨0, 2, 1, 0⟩]
 
-@[simp] instance : IsGeachLogic (𝐒𝟒.𝟐 : AxiomSet α) where taples := [⟨0, 0, 1, 0⟩, ⟨0, 2, 1, 0⟩, ⟨1, 1, 1, 1⟩].reverse
+instance : IsGeachLogic (α := α) 𝐒𝟒.𝟐 where taples := [⟨0, 0, 1, 0⟩, ⟨0, 2, 1, 0⟩, ⟨1, 1, 1, 1⟩]
 
-@[simp] instance : IsGeachLogic (𝐒𝟓 : AxiomSet α) where taples := [⟨0, 0, 1, 0⟩, ⟨1, 1, 0, 1⟩].reverse
+instance : IsGeachLogic (α := α) 𝐒𝟓 where taples := [⟨0, 0, 1, 0⟩, ⟨1, 1, 0, 1⟩]
 
-@[simp] instance : IsGeachLogic (𝐊𝐓𝟒𝐁 : AxiomSet α) where taples := [⟨0, 0, 1, 0⟩, ⟨0, 2, 1, 0⟩, ⟨0, 1, 0, 1⟩].reverse
+instance : IsGeachLogic (α := α) 𝐊𝐓𝟒𝐁 where taples := [⟨0, 0, 1, 0⟩, ⟨0, 2, 1, 0⟩, ⟨0, 1, 0, 1⟩]
 
 end AxiomSet
 
