Logic/Modal/Standard/Kripke/Reducible.lean
@@ -5,28 +5,29 @@ namespace LO.Modal.Standard
 
 namespace Kripke
 
-variable {W : Type*} {α : Type u} [DecidableEq α]
-variable {Λ₁ Λ₂ : AxiomSet α} {P₁ P₂ : ∀ {W : Type u}, [Inhabited W] → Frame W α → Prop}
-variable [hSound₁ : Sound Λ₁ 𝔽(Λ₁)] [hSound₂ : Sound Λ₂ 𝔽(Λ₂)]
-variable [hComp₁ : Complete Λ₁ 𝔽(Λ₁)] [hComp₂ : Complete Λ₂ 𝔽(Λ₂)]
-variable (hDef₁ : AxiomSetDefinability Λ₁ P₁) (hDef₂ : AxiomSetDefinability Λ₂ P₂)
+variable
+  {α : Type u} [DecidableEq α]
+  {Λ₁ Λ₂ : AxiomSet α} {P₁ P₂ : ∀ {W : Type u}, [Inhabited W] → Frame W α → Prop}
+  [sound₁ : Sound Λ₁ 𝔽(Λ₁)] [sound₂ : Sound Λ₂ 𝔽(Λ₂)]
+  [complete₁ : Complete Λ₁ 𝔽(Λ₁)] [complete₂ : Complete Λ₂ 𝔽(Λ₂)]
+  [definability₁ : Definability Λ₁ P₁] [definability₂ : Definability Λ₂ P₂]
 
-lemma reducible_of_subset_axiomSetFrameClass (hs : ∀ {W}, [hiW : Inhabited W] → ∀ {F}, 𝔽(Λ₂) W hiW F → 𝔽(Λ₁) W hiW F) : Λ₁ ≤ₛ Λ₂ := by
+lemma reducible_of_subset_axiomSetFrameClass (hs : ∀ {W}, [Inhabited W] → ∀ {F}, 𝔽(Λ₂) W F → 𝔽(Λ₁) W F) : Λ₁ ≤ₛ Λ₂ := by
   apply System.reducible_iff.mpr;
   intro p hp;
-  apply hComp₂.complete;
+  apply complete₂.complete;
   intro W _ F hF;
-  exact hSound₁.sound hp W F $ hs hF;
+  exact sound₁.sound hp W F $ hs hF;
 
 lemma reducible_of_definability (hs : ∀ {W}, [Inhabited W] → ∀ {F : Frame W α}, P₂ F → P₁ F) : Λ₁ ≤ₛ Λ₂ := by
   apply reducible_of_subset_axiomSetFrameClass;
-  intro W hiW F hF;
-  apply iff_definability_memAxiomSetFrameClass hDef₁ |>.mpr;
-  exact hs $ iff_definability_memAxiomSetFrameClass hDef₂ |>.mp hF;
+  intro W _ F hF;
+  apply iff_definability_memAxiomSetFrameClass definability₁ |>.mpr;
+  exact hs $ iff_definability_memAxiomSetFrameClass definability₂ |>.mp hF;
 
 lemma equiv_of_eq_axiomSetFrameClass
-  (hs₁ : ∀ {W}, [hiW : Inhabited W] → ∀ {F}, 𝔽(Λ₂) W hiW F → 𝔽(Λ₁) W hiW F)
-  (hs₂ : ∀ {W}, [hiW : Inhabited W] → ∀ {F}, 𝔽(Λ₁) W hiW F → 𝔽(Λ₂) W hiW F)
+  (hs₁ : ∀ {W}, [Inhabited W] → ∀ {F}, 𝔽(Λ₂) W F → 𝔽(Λ₁) W F)
+  (hs₂ : ∀ {W}, [Inhabited W] → ∀ {F}, 𝔽(Λ₁) W F → 𝔽(Λ₂) W F)
   : Λ₁ =ₛ Λ₂ := by
   apply System.Equiv.antisymm_iff.mpr;
   constructor;
@@ -36,9 +37,7 @@ lemma equiv_of_eq_axiomSetFrameClass
 lemma equiv_of_iff_definability (h : ∀ {W}, [Inhabited W] → ∀ {F : Frame W α}, P₁ F ↔ P₂ F) : Λ₁ =ₛ Λ₂ := by
   apply System.Equiv.antisymm_iff.mpr;
   constructor;
-  . apply reducible_of_definability hDef₁ hDef₂;
-    intros; apply h.mpr; assumption;
-  . apply reducible_of_definability hDef₂ hDef₁;
-    intros; apply h.mp; assumption;
+  . apply reducible_of_definability (definability₁ := definability₁) (definability₂ := definability₂); intros; exact h.mpr (by assumption)
+  . apply reducible_of_definability (definability₁ := definability₂) (definability₂ := definability₁); intros; exact h.mp (by assumption)
 
 end LO.Modal.Standard.Kripke
